Table-driven parser now uses Extraction Implicit to avoid constructing and computing with types everywhere.  It takes about 43 seconds on my laptop to build the parser table which seems to have 117 states.

x86model/Model/NewParser.v
@@ -52,8 +52,105 @@ Module Type NEW_PARSER_ARG.
   Variable token_id_to_chars : token_id -> list char_p.
 End NEW_PARSER_ARG.
 
-Module NewParser(PA : NEW_PARSER_ARG).
-Import PA.
+(* a module for generating the parser for x86 instructions *)
+Module X86_PARSER_ARG.
+  Require Import X86Syntax.
+  Require Import Bits.
+  Local Open Scope Z_scope.
+  
+  Definition char_p : Set := bool.
+  Definition char_dec : forall (c1 c2:char_p), {c1=c2}+{c1<>c2} := bool_dec.
+  Inductive type : Set := 
+  | Int_t : type
+  | Register_t : type
+  | Byte_t : type
+  | Half_t : type
+  | Word_t : type
+  | Double_Word_t : type
+  | Ten_Byte_t : type
+  | Scale_t : type
+  | Condition_t : type
+  | Address_t : type
+  | Operand_t : type
+  | Fpu_Register_t : type
+  | Fp_Debug_Register_t : type
+  | Fp_Operand_t : type 
+  | MMX_Granularity_t : type
+  | MMX_Register_t : type
+  | MMX_Operand_t : type
+  | SSE_Register_t : type
+  | SSE_Operand_t : type
+  | Instruction_t : type
+  | Control_Register_t : type
+  | Debug_Register_t : type
+  | Segment_Register_t : type
+  | Lock_or_Rep_t : type
+  | Bool_t : type
+  | Prefix_t : type
+  | Option_t (t: type) : type
+  (* Need pairs at this level if I want to have options of pairs*)
+  | UPair_t (t1 t2: type) : type. 
+
+  Definition tipe := type.
+  Definition tipe_eq : forall (t1 t2:tipe), {t1=t2} + {t1<>t2}.
+    intros ; decide equality.
+  Defined.
+
+  Fixpoint tipe_m (t:tipe) := 
+    match t with 
+      | Int_t => Z
+      | Register_t => register
+      | Byte_t => int8
+      | Half_t => int16
+      | Word_t => int32
+      | Double_Word_t => int64
+      | Ten_Byte_t => int80
+      | Scale_t => scale
+      | Condition_t => condition_type
+      | Address_t => address
+      | Operand_t => operand
+      | Fpu_Register_t => int3
+      | Fp_Debug_Register_t => fp_debug_register
+      | Fp_Operand_t => fp_operand  
+      | MMX_Granularity_t => mmx_granularity
+      | MMX_Register_t => mmx_register
+      | MMX_Operand_t => mmx_operand
+      | SSE_Register_t => sse_register
+      | SSE_Operand_t => sse_operand
+      | Instruction_t => instr
+      | Control_Register_t => control_register
+      | Debug_Register_t => debug_register
+      | Segment_Register_t => segment_register
+      | Lock_or_Rep_t => lock_or_rep
+      | Bool_t => bool
+      | Prefix_t => prefix
+      | Option_t t => option (tipe_m t)
+      | UPair_t t1 t2 => ((tipe_m t1) * (tipe_m t2))%type
+    end.
+  Definition user_type := type.
+  Definition user_type_dec : forall (t1 t2:user_type), {t1=t2} + {t1<>t2} := 
+    tipe_eq.
+  Definition user_type_denote := tipe_m.
+
+  Definition byte_explode (b:int8) : list bool := 
+  let bs := Word.bits_of_Z 8 (Word.unsigned b) in
+    (bs 7)::(bs 6)::(bs 5)::(bs 4)::(bs 3)::(bs 2)::(bs 1)::(bs 0)::nil.
+
+  Definition nat_explode (n:nat) : list bool := 
+    byte_explode (Word.repr (Z_of_nat n)).
+
+  Definition token_id := nat.
+  Definition num_tokens : token_id := 256%nat.
+  Definition token_id_to_chars : token_id -> list char_p := nat_explode.
+End X86_PARSER_ARG.
+
+(******************************************************************************)
+(* I would like to put this in a module but alas, the Extraction Implicit     *)
+(* stuff breaks then.  So I've had to break this out to top-level.            *)
+(******************************************************************************)
+(* Module X86_BASE_PARSER(NewParser(PA : NEW_PARSER_ARG). *)
+(*Import PA.*)
+Import X86_PARSER_ARG.
 
 (** The [type]s for our grammars -- later, we'll need to extend this with user-defined 
      types. *)
@@ -108,92 +205,60 @@ Inductive xform : type -> type -> Type :=
 .
 Notation "t1 ->> t2" := (xform t1 t2) (left associativity, at level 69, t2 at next level).
 
+(** These declarations ensure that the types will be erased upon extraction.
+    But we must make sure not to ever eliminate these types... *)
+Extraction Implicit Xid [t].
+Extraction Implicit Xzero [t].
+Extraction Implicit Xcomp [t1 t2 t3].
+Extraction Implicit Xchar [t].
+Extraction Implicit Xunit [t].
+Extraction Implicit Xempty [t1 t2].
+Extraction Implicit Xpair [t t1 t2].
+Extraction Implicit Xfst [t1 t2].
+Extraction Implicit Xsnd [t1 t2].
+Extraction Implicit Xinl [t1 t2].
+Extraction Implicit Xinr [t1 t2].
+Extraction Implicit Xmatch [t1 t2 t].
+Extraction Implicit Xcons [t1 t2].
+Extraction Implicit Xmap [t1 t2].
+
 (** Interpret an [t1 ->> t2] xform as a function [interp t1 -> interp t2]. *)
 Fixpoint xinterp t1 t2 (x: t1 ->> t2) : interp t1 -> interp t2 := 
   match x in t1 ->> t2 return interp t1 -> interp t2 with 
     | Xid t => fun (x:interp t) => x
     | Xzero t => fun (x:interp Void_t) => match x with end
-    | Xcomp t1 t2 t3 f1 f2 => fun (x:interp t1) => xinterp f2 (xinterp f1 x)
+    | Xcomp t1 t2 t3 f1 f2 => 
+      let f1' := xinterp f1 in 
+        let f2' := xinterp f2 in 
+          fun (x:interp t1) => f2' (f1' x)
     | Xchar t c => fun (x:interp t) => c
     | Xunit t => fun (x:interp t) => tt
     | Xempty t1 t2 => fun (x:interp t1) => @nil (interp t2)
-    | Xpair t t1 t2 f1 f2 => fun (x:interp t) => (xinterp f1 x, xinterp f2 x)
+    | Xpair t t1 t2 f1 f2 => 
+      let f1' := xinterp f1 in 
+        let f2' := xinterp f2 in 
+          fun (x:interp t) => (f1' x, f2' x)
     | Xfst t1 t2 => fun (x:interp (Pair_t t1 t2)) => fst x
     | Xsnd t1 t2 => fun (x:interp (Pair_t t1 t2)) => snd x
     | Xinl t1 t2 => fun (x:interp t1) => inl (interp t2) x
     | Xinr t1 t2 => fun (x:interp t2) => inr (interp t1) x
     | Xmatch t1 t2 t f1 f2 => 
+      let f1' := xinterp f1 in 
+        let f2' := xinterp f2 in 
       fun (x:interp (Sum_t t1 t2)) => 
         match x with 
-          | inl x1 => xinterp f1 x1
-          | inr x2 => xinterp f2 x2
+          | inl x1 => f1' x1 
+          | inr x2 => f2' x2 
         end
-    | Xcons t1 t2 f1 f2 => fun (x:interp t1) => (xinterp f1 x)::(xinterp f2 x)
-    | Xmap t1 t2 f => fun (x:interp (List_t t1)) => List.map (xinterp f) x
+    | Xcons t1 t2 f1 f2 => 
+      let f1' := xinterp f1 in 
+        let f2' := xinterp f2 in 
+          fun (x:interp t1) => (f1' x)::(f2' x)
+    | Xmap t1 t2 f => 
+      let f' := xinterp f in 
+        fun (x:interp (List_t t1)) => List.map f' x
   end.
-
-(** * Decidable equality for [xform]'s. *)
-Lemma existT_neq (A:Type) (P:A->Type) (x y:A) (vx:P x) (vy:P y) : 
-  x <> y -> (existT P x vx) <> (existT P y vy).
-Proof.
-  intros. intro. apply (simplification_existT1 _ P _ x y vx vy) ; auto.
-Qed.
-
-Definition type_pair_dec (p1 p2:type*type) : {p1=p2} + {p1<>p2}.
-  intros. destruct p1. destruct p2. destruct (type_dec t t1) ; subst ;
-  [ destruct (type_dec t0 t2) ; subst ; [left | right ] | right ] ; 
-  congruence.
-Defined.
-
-Definition xform_dec' t1 t2 (x:t1 ->> t2) t3 t4 (y:t3 ->> t4) : 
-  {@existT (type*type)%type (fun p => fst p ->> snd p) (t1,t2) x = 
-   @existT (type*type)%type (fun p => fst p ->> snd p) (t3,t4) y}
-+ {@existT (type*type)%type (fun p => fst p ->> snd p) (t1,t2) x <> 
-   @existT (type*type)%type (fun p => fst p ->> snd p) (t3,t4) y}.
-Proof.
-  Ltac xdec := 
-    match goal with 
-      | [ H : existT ?f ?t ?x = existT ?f ?t ?y |- _ ] => 
-        generalize (inj_pairT2 _ f t x y H) ; clear H ; intro H ; subst 
-      | [ H : List_t _ = List_t _ |- _ ] => injection H ; clear H ; intros ; subst
-      | [ H : Pair_t _ _ = Pair_t _ _ |- _ ] => injection H ; clear H ; intros ; subst
-      | [ H : Sum_t _ _ = Sum_t _ _ |- _ ] => injection H ; clear H ; intros ; subst
-      | _ => idtac
-    end.
-  intros. destruct (type_pair_dec (t1,t2) (t3,t4)) ; 
-  [idtac | right ; apply existT_neq ; auto]. injection e. clear e.
-  generalize t3 t4 y ; clear t3 t4 y. induction x ; destruct y ; intros ; repeat xdec ; 
-  try (subst ; congruence) ; try (subst ; left ; auto ; fail) ; 
-  repeat subst ; try (right ; intro ; xdec ; discriminate).
-   destruct (type_dec t2 t4). subst. specialize (IHx1 _ _ y1 (eq_refl _) (eq_refl _)).
-   specialize (IHx2 _ _ y2 (eq_refl _) (eq_refl _)). 
-   destruct IHx1 ; [ destruct IHx2 ; [left | right ] | right] ; repeat xdec ; auto.
-   intro. xdec. injection H. intros. xdec. xdec. apply n ; auto.
-   intro. xdec. injection H. intros. xdec. xdec. apply n ; auto.
-   right. intro. xdec. injection H. intros. repeat xdec. congruence.
-   destruct (char_dec c c0). subst. left. auto. right. intro. xdec.
-   injection H0. auto. specialize (IHx1 _ _ y1 (eq_refl _) (eq_refl _)).
-   specialize (IHx2 _ _ y2 (eq_refl _) (eq_refl _)).  
-   destruct IHx1 ; [ destruct IHx2 ; [ left | right ] | right] ; repeat xdec ; auto.
-   intro ; xdec. injection H ; intros ; repeat xdec. apply n ; auto.
-   intro ; xdec. injection H ; intros ; repeat xdec. apply n ; auto.
-   specialize (IHx1 _ _ y1 (eq_refl _) (eq_refl _)). 
-   specialize (IHx2 _ _ y2 (eq_refl _) (eq_refl _)). 
-   destruct IHx1 ; destruct IHx2 ; try (left ; repeat xdec ; auto ; fail) ; 
-     right ; xdec ; intro ; xdec ; injection H ; intros ; subst ; repeat xdec ; 
-   apply n ; auto. specialize (IHx1 _ _ y1 (eq_refl _) (eq_refl _)).
-   specialize (IHx2 _ _ y2 (eq_refl _) (eq_refl _)). 
-   destruct IHx1 ; [ destruct IHx2 ; [left | right ] | right ] ; repeat xdec ; auto ; 
-     intro H ; repeat xdec ; injection H ; intros ; subst ; repeat xdec ; apply n ; auto.
-   specialize (IHx _ _ y (eq_refl _) (eq_refl _)). destruct IHx ; [left | right ] ; 
-   repeat xdec ; auto. intro. xdec. injection H ; intros ; subst. repeat xdec.
-   apply n ; auto.
-Defined.
-
-Definition xform_dec t1 t2 (x1 x2:t1 ->> t2) : {x1 = x2} + {x1 <> x2}.
-  intros. destruct (xform_dec' x1 x2). xdec. left. auto. right.
-  intro. subst. apply n. auto.
-Defined.
+Extraction Implicit xinterp [t1 t2].
 
 (** * Grammars *)
 (** Our user-facing [grammar]s, indexed by a [type], reflecting the type of the
@@ -208,6 +273,12 @@ Inductive grammar : type -> Type :=
 | Star : forall t, grammar t -> grammar (List_t t)
 | Map : forall t1 t2, (interp t1 -> interp t2) -> grammar t1 -> grammar t2
 | Xform : forall t1 t2, t1 ->> t2 -> grammar t1 -> grammar t2.
+Extraction Implicit Zero [t].
+Extraction Implicit Cat [t1 t2].
+Extraction Implicit Alt [t1 t2].
+Extraction Implicit Star [t].
+Extraction Implicit Map [t1 t2].
+Extraction Implicit Xform [t1 t2].
 
 (** * Denotation of Grammars *)
 (** I'm a little annoyed that I had to break out so many equalities, but
@@ -238,6 +309,7 @@ Hint Constructors in_grammar.
 Definition xcoerce t1 t2 t3 t4 (x:xform t1 t2) : t1 = t3 -> t2 = t4 -> xform t3 t4.
   intros. subst. apply x.
 Defined.
+Extraction Implicit xcoerce [t1 t2 t3 t4].
 Definition eq_pair_fst t1 t2 t3 t4 : (Pair_t t1 t2 = Pair_t t3 t4) -> t3 = t1.
   intros ; injection H. intros. apply (eq_sym H1).
 Defined.
@@ -267,31 +339,33 @@ Definition xpair_fst ta tc (x2:ta->>tc):forall t1 t2,
     | Xsnd t3 t4 => fun t1 t2 H => xcoerce (Xid _) (eq_sym H) (pair_eq_snd H)
     | x2 => fun t1 t2 H => Xpair (xcoerce (Xfst t1 t2) (eq_sym H) (eq_refl _)) x2
   end.
+Extraction Implicit xpair_fst [ta tc t1 t2].
+
+Definition xpair_r ta tb tc (x2:ta ->> tc) : (ta ->> tb) -> ta ->> (Pair_t tb tc) := 
+  match x2 in ta ->> tc return ta->>tb -> ta->>(Pair_t tb tc) with
+    | Xzero _ => fun x1 => Xzero _
+    | x2 => fun x1 => Xpair x1 x2
+  end.
+Extraction Implicit xpair_r [ta tb tc].
 
 Definition xpair ta tb tc (x1:ta ->> tb) (x2:ta ->> tc) : ta ->> (Pair_t tb tc) := 
  match x1 in ta ->> tb return ta->>tc -> ta->>(Pair_t tb tc) with
    | Xfst t1 t2 => fun x2 => xpair_fst x2 (eq_refl _)
-   | x1 => Xpair x1
+   | Xzero t => fun x2 => Xzero _
+   | x1 => fun x2 => xpair_r x2 x1 
   end x2.
+Extraction Implicit xpair [ta tb tc].
 
 (** The [xpair] optimization preserves meaning. *)
 Lemma xpair_corr ta tb tc (x1:ta->>tb) (x2:ta->>tc) v : 
   xinterp (xpair x1 x2) v = xinterp (Xpair x1 x2) v.
 Proof.
-  destruct x1 ; simpl ; auto. intros. dependent destruction x2 ; simpl ; auto.   
+  Ltac xpair_corr_simp := 
+    match goal with | [ H : void |- _ ] => destruct H | _ => auto end.  
+  destruct x1 ; simpl in * ; auto ; intros ; xpair_corr_simp ; 
+  dependent destruction x2 ; simpl in * ; xpair_corr_simp.
   destruct v. auto.
 Qed.
-
-(*
-Definition xmatch_inl tb tc (x2:tb->>tc) : forall t1 t2, tc = Sum_t t1 t2 -> 
-  Sum_t t1 tb ->> tc.
-refine (fun tb tc x2 => 
-  match x2 in tb->>tc return forall t1 t2, tc=Sum_t t1 t2 -> Sum_t t1 tb ->> tc with
-    | Xinr t3 t4 => fun t1 t2 H => _
-    | x2 => fun t1 t2 H => _
-  end
-).*)
-
 
 Definition xmatch_inl t1 t2 tb tc (x2:tb->>tc) : 
   (tc=Sum_t t1 t2) -> Sum_t t1 tb ->> Sum_t t1 t2.
@@ -302,6 +376,7 @@ refine (fun t1 t2 tb tc x2 =>
   end
 ). injection H ; intros ; subst. auto.
 Defined.
+Extraction Implicit xmatch_inl [t1 t2 tb tc].
 
 (** This function and the two above implement the reduction
     [match x with inl a => inl a | inr b => inr b end = id]. *)
@@ -310,6 +385,7 @@ Definition xmatch ta tb tc (x1:ta->>tc) (x2:tb->>tc) : Sum_t ta tb ->> tc :=
     | Xinl t1 t2 => fun x2' => xmatch_inl x2' (eq_refl _)
     | x1' => Xmatch x1'
   end x2.
+Extraction Implicit xmatch [ta tb tc].
 
 (** Correctness of eta-reduction for sums. *)
 Lemma xmatch_corr ta tb tc (x1:ta->>tc) (x2:tb->>tc) v : 
@@ -321,29 +397,16 @@ Qed.
 
 (** These next few functions implement specific reductions for when a particular
     combinator is composed with another.  Together, they implement the cut
-    elimination for the sequent language. *)
+    elimination for the sequent language. 
+*)
 (** (f1, f2) o id = (f1, f2)
     (f1, f2) o (char c) = char c
     (f1, f2) o unit = unit
     (f1, f2) o empty = empty
-    (f1, f2) o (fst f) = f1 o f
-    (f1, f2) o (snd f) = f2 o f
-
-    (f1, f2) o (fst o g1, snd o g2) = (f1 o g1, f2 o g2) ?
+    (f1, f2) o fst = f1
+    (f1, f2) o snd = f2
+    (f1, f2) o (g1, g2) = ((f1, f2) o g1, (f1, f2) o g2)
 *)
-
-(*
-Definition xcomp_pair_pair_fst_snd 
-  t t1 (f1:t ->> t1) t2 (f2:t ->> t2)
-  t3 (g1 : t1 ->> t3) t4 (g2: t2 ->> t4) : t ->> (Pair_t t3 t4) := 
-  (Xcomp (Xpair f1 f2) (Xpair (Xcomp (Xfst _ (Xid _)) g1) (Xcomp (Xsnd _ (Xid _)) g2))).
-
-Definition opt_xcomp_pair_pair_fst_snd 
-  t t1 (f1:t ->> t1) t2 (f2:t ->> t2)
-  t3 (g1 : t1 ->> t3) t4 (g2: t2 ->> t4) : t ->> (Pair_t t3 t4) := 
-  (Xpair (Xcomp f1 g1) (Xcomp f2 g2)).
-*)
-
 Definition xcomp_pair t21 t22 (x2:t21 ->> t22) : 
   forall ta tb tc (x11:ta->>tb) (x12:ta->>tc), (Pair_t tb tc = t21) -> ta ->> t22 := 
     match x2 in t21 ->> t22 return
@@ -356,10 +419,15 @@ Definition xcomp_pair t21 t22 (x2:t21 ->> t22) :
         fun ta tb tc x11 x12 H => xcoerce x11 (eq_refl _) (eq_pair_fst (eq_sym H))
       | Xsnd te tf => 
         fun ta tb tc x11 x12 H => xcoerce x12 (eq_refl _) (eq_pair_snd (eq_sym H))
+      | Xpair u1 u2 u3 x21 x22 => 
+        fun ta tb tc x11 x12 H => 
+          Xpair (Xcomp (Xpair x11 x12) (xcoerce x21 (eq_sym H) (eq_refl _))) 
+                (Xcomp (Xpair x11 x12) (xcoerce x22 (eq_sym H) (eq_refl _)))
       | x2' => 
         fun ta tb tc x11 x12 H => 
           Xcomp (Xpair x11 x12) (xcoerce x2' (eq_sym H) (eq_refl _))
     end.
+Extraction Implicit xcomp_pair [t21 t22 ta tb tc].
 
 (** [xcomp_pair] is correct. *)
 Lemma xcomp_pair_corr t21 t22 (x2:t21->>t22) ta tb tc (x11:ta->>tb) (x12:ta->>tc) H v: 
@@ -389,6 +457,7 @@ Definition xcomp_inl t21 t22 (x2:t21 ->> t22) :
       | x2' => 
         fun ta tb H => Xcomp (Xinl _ _) (xcoerce x2' (eq_sym H) (eq_refl _))
     end.
+Extraction Implicit xcomp_inl [t21 t22 ta tb].
 
 (** [xcomp_inl] is correct *)
 Lemma xcomp_inl_corr t21 t22 (x2:t21->>t22) ta tb (H:Sum_t ta tb = t21) v: 
@@ -418,6 +487,7 @@ Definition xcomp_inr t21 t22 (x2:t21 ->> t22) :
       | x2' => 
         fun ta tb H => Xcomp (Xinr _ _) (xcoerce x2' (eq_sym H) (eq_refl _))
     end.
+Extraction Implicit xcomp_inr [t21 t22 ta tb].
 
 (** [xcomp_inr] is correct. *)
 Lemma xcomp_inr_corr t21 t22 (x2:t21->>t22) ta tb (H:Sum_t ta tb = t21) v: 
@@ -448,6 +518,7 @@ Definition xcomp_map t21 t22 (x2:t21 ->> t22) :
       | x2' => 
           fun ta tb x11 H => Xcomp (Xmap x11) (xcoerce x2' (eq_sym H) (eq_refl _))
     end.
+Extraction Implicit xcomp_map [t21 t22 ta tb].
 
 (** [xcomp_map] is correct. *)
 Lemma xcomp_map_corr t21 t22 (x2:t21->>t22) ta tb (x11:ta->>tb) (H:List_t tb = t21) v : 
@@ -475,6 +546,7 @@ Definition xcomp_empty t21 t22 (x2:t21 ->> t22) :
       | Xmap tc td f => fun ta tb H => Xempty _ _
       | x2' => fun ta tb H => Xcomp (Xempty _ _) (xcoerce x2' (eq_sym H) (eq_refl _))
     end.
+Extraction Implicit xcomp_empty [t21 t22 ta tb].
 
 (** [xcomp_empty] is correct. *)
 Lemma xcomp_empty_corr t21 t22 (x2:t21->>t22) ta tb (H:List_t tb = t21) v : 
@@ -505,6 +577,7 @@ Definition xcomp_cons t21 t22 (x2:t21 ->> t22) :
       | x2' => fun ta tb x11 x21 H => 
         Xcomp (Xcons x11 x21) (xcoerce x2' (eq_sym H) (eq_refl _))
     end.
+Extraction Implicit xcomp_cons [t21 t22 ta tb].
 
 (** [xcomp_cons] is correct. *)
 Lemma xcomp_cons_corr t21 t22 (x2:t21->>t22) ta tb (x11:ta->>tb) (x12:ta->>List_t tb) H v: 
@@ -530,6 +603,7 @@ Definition xcomp_r t21 t22 (x2:t21 ->> t22) : forall t11, t11 ->> t21 -> t11 ->>
     | Xpair t t21 t22 x21 x22 => fun t1 x1 => Xpair (Xcomp x1 x21) (Xcomp x1 x22)
     | x2' => fun t1 x1 => Xcomp x1 x2'
   end.
+Extraction Implicit xcomp_r [t21 t22 t11].
 
 (** [xcomp_r] is correct. *)
 Lemma xcomp_r_corr t21 t22 (x2:t21->>t22) t11 (x1:t11->>t21) v : 
@@ -542,6 +616,7 @@ Qed.
      id o f = f
      zero o f = zero
      (f1 o f2) o f3 = f1 o (f2 o f3)
+     (match f1 f2) o f3 = match (f1 o f3) (f2 o f3)
      plus the reductions in the functions above
 *)
 Fixpoint xcomp t11 t12 (x1:t11 ->> t12) : forall t22, t12 ->> t22 -> t11 ->> t22 := 
@@ -557,8 +632,10 @@ Fixpoint xcomp t11 t12 (x1:t11 ->> t12) : forall t22, t12 ->> t22 -> t11 ->> t22
       | Xmap ta tb x11 => fun t22 x2 => xcomp_map x2 x11 (eq_refl _)
       | Xempty ta tb => fun t22 x2 => xcomp_empty x2 _ (eq_refl _)
       | Xcons ta tb x11 x12 => fun t22 x2 => xcomp_cons x2 x11 x12 (eq_refl _)
+      | Xmatch ta tb tc x11 x12 => fun t22 x2 => Xmatch (xcomp x11 x2) (xcomp x12 x2)
       | x1' => fun t22 x2 => xcomp_r x2 x1'
     end.
+Extraction Implicit xcomp [t11 t12 t22].
 
 (** [xcomp] (cut elimination) is correct. *)
 Lemma xcomp_corr t1 t2 (x1:t1->>t2) t3 (x2:t2->>t3) v : 
@@ -572,7 +649,8 @@ Proof.
   end.
   simpl in *. rewrite <- IHx1_2. rewrite <- IHx1_1. auto.
   apply xcomp_empty_corr. apply xcomp_pair_corr.  apply xcomp_inl_corr.
-  apply xcomp_inr_corr. apply xcomp_cons_corr. apply xcomp_map_corr.
+  apply xcomp_inr_corr. destruct v ; auto. rewrite IHx1_1. auto. rewrite IHx1_2. auto.
+  apply xcomp_cons_corr. apply xcomp_map_corr.
 Qed.
 
 Fixpoint xcomp' tb tc (x2:tb->>tc) : forall ta, ta->>tb -> ta->>tc := 
@@ -581,6 +659,7 @@ Fixpoint xcomp' tb tc (x2:tb->>tc) : forall ta, ta->>tb -> ta->>tc :=
     | Xpair td te tf x21 x22 => fun ta x1 => Xpair (xcomp' x21 x1) (xcomp' x22 x1)
     | x2' => fun ta x1 => xcomp x1 x2'
   end.
+Extraction Implicit xcomp' [tb tc ta].
 
 Lemma xcomp'_corr tb tc (x2:tb->>tc) ta (x1:ta->>tb) v : 
   xinterp (xcomp' x2 x1) v = xinterp (Xcomp x1 x2) v.
@@ -602,6 +681,7 @@ Fixpoint xopt t1 t2 (x:t1 ->> t2) : t1 ->> t2 :=
     | Xmap ta tb x1 => Xmap (xopt x1)
     | x' => x'
   end.
+Extraction Implicit xopt [t1 t2].
 
 (** [xopt] is correct. *)
 Lemma xopt_corr t1 t2 (x:t1 ->> t2) : xinterp (xopt x) = xinterp x.
@@ -619,6 +699,7 @@ Definition OptAlt_r t2 (g2:grammar t2) : forall t1, grammar t1 -> grammar (Sum_t
     | Zero t2 => fun t1 g1 => Xform (Xinl _ _) g1
     | g2' => fun t1 g1 => Alt g1 g2'
   end.
+Extraction Implicit OptAlt_r [t2 t1].
 
 (** 0 ++ g ==> g @ inr *)
 Definition OptAlt_l t1 (g1:grammar t1) : forall t2, grammar t2 -> grammar (Sum_t t1 t2) :=
@@ -626,10 +707,12 @@ Definition OptAlt_l t1 (g1:grammar t1) : forall t2, grammar t2 -> grammar (Sum_t
     | Zero t1 => fun t2 g2 => Xform (Xinr _ _) g2
     | g1' => fun t2 g2 => OptAlt_r g2 g1'
   end.
+Extraction Implicit OptAlt_l [t1 t2].
 
 (** Should reduce (g ++ g) ==> g and perhaps re-order according to some
     total order on the grammars. *)
 Definition OptAlt t1 t2 (g1:grammar t1) (g2:grammar t2) := OptAlt_l g1 g2.
+Extraction Implicit OptAlt [t1 t2].
 
 (** g $ 0 ==> 0 @ zero_to_t
     g $ eps ==> g @ add_unit_r *)
@@ -639,6 +722,7 @@ Definition OptCat_r t2 (g2:grammar t2) : forall t1, grammar t1 -> grammar (Pair_
     | Eps => fun t1 (g1 : grammar t1) => Xform (Xpair (Xid _) (Xunit _)) g1
     | g2' => fun t1 (g1 : grammar t1) => Cat g1 g2'
   end.
+Extraction Implicit OptCat_r [t2 t1].
 
 (** 0 $ g ==> 0 @ zero_to_t
     eps $ g ==> g @ add_unit_l *)
@@ -648,6 +732,7 @@ Definition OptCat t1 (g1:grammar t1) : forall t2, grammar t2 -> grammar (Pair_t 
     | Eps => fun t2 (g2 : grammar t2) => Xform (Xpair (Xunit _) (Xid _)) g2
     | g1' => fun t2 (g2 : grammar t2) => OptCat_r g2 g1'
   end.
+Extraction Implicit OptCat [t1 t2].
 
 (** star (star g) ==> (star g) @ mklist
     star eps ==> eps @ to_empty_list
@@ -660,6 +745,7 @@ Definition OptStar t (g:grammar t) : grammar (List_t t) :=
     | Zero t => Xform (Xempty _ _) Eps
     | g' => Star g'
   end.
+Extraction Implicit OptStar [t].
 
 (** 0 @ f ==> 0
     g @ f1 @ f2 ==> g @ (f1 o f2)
@@ -670,9 +756,11 @@ Definition OptMap' t1 (g:grammar t1) : forall t2, (interp t1 -> interp t2) -> gr
     | Map u1 u2 f' g' => fun t2 f => @Map u1 t2 (fun x => f (f' x)) g'
     | g' => fun t2 f => @Map _ t2 f g'
   end.
+Extraction Implicit OptMap' [t1 t2].
 
 Definition OptMap t1 t2 (f:interp t1 -> interp t2) (g:grammar t1) : grammar t2 := 
   @OptMap' t1 g t2 f.
+Extraction Implicit OptMap [t1 t2].
 
 Definition OptXform' t1 (g:grammar t1) : forall t2, t1->>t2 -> grammar t2 :=
   match g in grammar t1' return forall t2, t1'->>t2 -> grammar t2 with
@@ -680,8 +768,10 @@ Definition OptXform' t1 (g:grammar t1) : forall t2, t1->>t2 -> grammar t2 :=
     | Xform u1 u2 x' g' => fun t2 x => Xform (xcomp x' x) g'
     | g' => fun t2 x => Xform x g'
   end.
+Extraction Implicit OptXform' [t1 t2].
 
 Definition OptXform t1 t2 (x:t1->>t2) (g:grammar t1) := @OptXform' t1 g t2 x.
+Extraction Implicit OptXform [t1 t2].
 
 (** Generic simplification tactic. *)
 Ltac mysimp := 
@@ -818,6 +908,7 @@ Fixpoint null t (g:grammar t) : grammar t :=
     | Xform t1 t2 x g => OptXform x (null g)
     | Star t g => Xform (Xempty _ _) Eps
   end.
+Extraction Implicit null [t].
 
 (** Computes the derivative of [g] with respect to [c]. Denotationally,
     this is { (s,v) | (c::s,v) in_grammar[g] }. *)
@@ -836,6 +927,7 @@ Fixpoint deriv t (g:grammar t) (c:char_p) : grammar t :=
     | Star t g => 
         OptXform (Xcons (Xfst _ _) (Xsnd _ _)) (OptCat (deriv g c) (Star g))
   end.
+Extraction Implicit deriv [t].
 
 (** * AST Grammars *)
 
@@ -894,6 +986,7 @@ Definition fixfn (ag:astgram) (t:type) := interp (astgram_type ag) -> interp t.
 Definition ag_and_fn (t:type) (ag:astgram) (f:fixfn ag t) : { ag : astgram & fixfn ag t } :=
   existT (fun ag => fixfn ag t) ag f.
 Implicit Arguments ag_and_fn [t].
+Extraction Implicit ag_and_fn [t].
 
 (** Split a [grammar] into a simplified [astgram] (with no maps) and a top-level fix-up
     function that can turn the results of the [astgram] back into the user-specified 
@@ -927,6 +1020,7 @@ Fixpoint split_astgram t (g:grammar t) : { ag : astgram & fixfn ag t} :=
       let (ag, f2) := split_astgram g in 
         ag_and_fn ag (fun x => (xinterp f) (f2 x))
   end.
+Extraction Implicit split_astgram [t].
 
 (** Inversion principles for [astgram]s. *)
 Lemma inv_aeps : forall s v, in_astgram aEps s v -> s = nil /\ v = tt.
@@ -1023,6 +1117,7 @@ Qed.
 
 Definition agxf (t:type) (ag:astgram) (f:astgram_type ag ->> t) : 
   {ag : astgram & astgram_type ag ->> t} := existT _ ag f.
+Extraction Implicit agxf [t].
 
 (** Flatten out and right-associate a list of [aAlt]s. *)
 Fixpoint append_alt (ag1:astgram) (ag2:astgram) : 
@@ -1103,6 +1198,7 @@ Definition opt_ag (ag:astgram) : {ag2:astgram & astgram_type ag2 ->> astgram_typ
 Definition cast_interp t1 (v:interp (astgram_type t1)) t2 (H:t1 = t2) : interp (astgram_type t2).
   intros. rewrite <- H. apply v.
 Defined.
+Extraction Implicit cast_interp [t1 t2].
 
 Lemma astar_azero : forall ag cs v (H1:in_astgram ag cs v) (H2:ag = aStar aZero),
   cs = nil /\ @cast_interp ag v _ H2 = nil.
@@ -1145,6 +1241,7 @@ Qed.
 (** Optimize the [astgram] and optimize the resulting [xform]. *)
 Definition opt_agxf (t:type) (ag:astgram) (f:astgram_type ag ->> t) := 
   let (ag', f') := opt_ag ag in agxf ag' (xcomp f' f).
+Extraction Implicit opt_agxf [t].
 
 Lemma opt_agxf_corr1 t ag (f:astgram_type ag ->> t) cs v : 
   in_agxf (existT _ ag f) cs v -> in_agxf (opt_agxf ag f) cs v.
@@ -1557,7 +1654,7 @@ Fixpoint derivs_and_split (ag:astgram) (cs:list char_p) :
     | nil => agxf ag (Xid _)
     | c::cs' => let (ag1, x1) := deriv_and_split ag c in 
                 let (ag2, x2) := derivs_and_split ag1 cs' in 
-                  agxf ag2 (xcomp' x1 x2)
+                  agxf ag2 (xopt (xcomp' x1 x2))
   end.
 
 Lemma derivs_and_split_corr1 cs ag v : 
@@ -1567,9 +1664,10 @@ Proof.
   generalize (deriv_and_split_corr1 H). intros. specialize (H0 _ _ (eq_refl _)).
   unfold in_agxf in *. destruct (deriv_and_split ag a). mysimp. 
   remember (derivs_and_split x cs) as e. destruct e. 
-  unfold agxf. specialize (IHcs _ _ H0). rewrite <- Heqe in IHcs. mysimp. 
+  unfold agxf. 
+  specialize (IHcs _ _ H0). rewrite <- Heqe in IHcs. mysimp. 
   subst. generalize (xcomp'_corr x0 x3 x4). intros.
-  exists x4. split ; auto.
+  exists x4. split ; auto. rewrite xopt_corr. auto.
 Qed.
 
 Lemma derivs_and_split_corr2 cs ag v : 
@@ -1579,7 +1677,8 @@ Proof.
   intros. generalize (deriv_and_split_corr2 ag a). intros.
   remember (deriv_and_split ag a) as e ; destruct e.  
   remember (derivs_and_split x cs) as e2 ; destruct e2. 
-  unfold in_agxf in H. unfold agxf in H. mysimp. eapply H0.
+  unfold in_agxf in H. unfold agxf in H. mysimp. rewrite xopt_corr in H1.
+  eapply H0.
   generalize (xcomp'_corr x0 x2 x3). intros. rewrite H2 in H1. simpl in H1.
   unfold in_agxf in IHcs. specialize (IHcs x). 
   rewrite <- Heqe2 in IHcs. subst. exists (xinterp x2 x3). split ; auto.
@@ -1596,6 +1695,7 @@ Definition parse t (g:grammar t) (cs : list char_p) : list (interp t) :=
   let (ag, fuser) := split_astgram g in 
     let (agfinal, xfinal) := derivs_and_split ag cs in 
     List.map (fun x => fuser (xinterp xfinal x)) (astgram_extract_nil agfinal).
+Extraction Implicit parse [t].
 
 Lemma parse_corr1 : forall t (g:grammar t) cs v, in_grammar g cs v -> In v (parse g cs).
 Proof.
@@ -1634,7 +1734,7 @@ Section DFA.
   Record entry_t(row:nat)(states:states_t) := 
     { next_state : nat ; 
       next_state_lt : next_state < length states ; 
-      next_xform : astgram_type (states.[next_state]) ->> astgram_type (states.[row])
+      next_xform : interp (astgram_type (states.[next_state])) -> interp (astgram_type (states.[row])) 
     }.
 
   Definition row_t(i:nat)(s:states_t) := list (entry_t i s).
@@ -1833,6 +1933,12 @@ Section DFA.
   Definition build_reject_table (s:states_t) : list bool := 
     List.map always_rejects s.
 
+  (** Abstract this development over the derivs_and_split function so we
+      can plug in a different version below. *)
+  Section ABS_DERIVS_AND_SPLIT.
+    Variable derivs : forall (ag:astgram)(cs:list char_p), 
+      {ag2:astgram & astgram_type ag2 ->> astgram_type ag}.
+
   (** Generate the transition matrix row for the state corresponding to the
       astgram [g].  In general, this will add new states. *)
   Section GENROW.
@@ -1849,13 +1955,13 @@ Section DFA.
         match n with 
           | 0 => existT _ nil nil
           | S n' => 
-            let (g',x) := derivs_and_split g (token_id_to_chars tid) in
+            let (g',x) := derivs g (token_id_to_chars tid) in
               let p := find_or_add g' s in 
                 let (s2, row) := gen_row' n' (s ++ (fst p)) (1 + tid) _ _ in 
                   let e : entry_t gpos ((s ++ (fst p)) ++ s2) := 
                     {| next_state := (snd p) ; 
                        next_state_lt := _ ; 
-                       next_xform := (xcoerce x _ _) |} in
+                       next_xform := xinterp (xcoerce x _ _) |} in
                     existT _ ((fst p) ++ s2) _
         end). rewrite nth_lt ; auto. rewrite app_length. omega.
       generalize (find_index_some g' s).
@@ -1879,9 +1985,9 @@ Section DFA.
     refine (
       {| next_state := next_state e ; 
          next_state_lt := app_length_lt s s1 (next_state_lt e) ; 
-         next_xform := xcoerce (next_xform e) _ _
+         next_xform := _ (next_xform e) 
       |}
-    ) ; rewrite app_nth1 ; auto. apply (next_state_lt e). 
+    ). rewrite app_nth1. rewrite nth_lt ; auto. apply (next_state_lt e).
   Defined.
 
   Definition coerce_transitions s1 s (ts:transitions_t s) : transitions_t (s ++ s1) := 
@@ -2064,11 +2170,14 @@ Section DFA.
     intros. rewrite H. auto.
   Qed.
 
+(*
   Definition lookup_trans (d:DFA) (row : nat) (col : nat) : 
-    option { ag : astgram & astgram_type ag ->> astgram_type (dfa_states d .[row]) } := 
+    option { ag : astgram & 
+      interp (astgram_type ag) -> interp (astgram_type (dfa_states d .[row])) } := 
     match nth_error (dfa_transition d) row as x return 
       match x with | Some r => row_num r = row | None => True end ->
-      option { ag : astgram & astgram_type ag ->> astgram_type (dfa_states d .[row])}
+      option { ag : astgram & 
+        interp (astgram_type ag) -> interp (astgram_type (dfa_states d .[row]))}
       with
       | None => fun _ => None
       | Some r => fun H => 
@@ -2079,7 +2188,6 @@ Section DFA.
         end
     end (dfa_transition_r d row).
     
-(*
   Lemma gen_row_is_deriv g gpos n s tid H H1 : 
     match gen_row' n s tid H H1 with 
       | existT s' r => 
@@ -2115,9 +2223,13 @@ Section DFA.
     Variable d : DFA.
     Variable t : type.
 
+    Definition coerce_dom (A A':type) (H:A=A') (B:Type) (f:interp A->B) : interp A' -> B.
+      intros A A' H. rewrite H. apply (fun B (f:interp A'->B) => f).
+    Defined.
+
     Fixpoint table_parse' (i:nat) (ts:list token_id) 
-      (f:astgram_type ((dfa_states d).[i]) ->> t) : 
-      option { a : astgram & ((astgram_type a ->> t) * (list token_id))%type } := 
+      (f:interp (astgram_type ((dfa_states d).[i])) -> interp t) : 
+      option { a:astgram & ((interp (astgram_type a) -> interp t) * (list token_id))%type } := 
         if nth i (dfa_accepts d) false then
           (* we are in an accepting state -- since this is shortest match, stop here *)
           Some (existT _ ((dfa_states d).[i])  (f, ts))
@@ -2143,11 +2255,16 @@ Section DFA.
                            compose the entry [e]'s [xform] with our accumulated
                            [xform]. *)
                         fun H' => table_parse' (next_state e) ts' 
-                          (xcomp (next_xform e) (xcoerce f (table_cast _ _ H) (eq_refl _)))
+                          (fun x => (coerce_dom (table_cast _ _ H) f) ((next_xform e) x))
                     end (eq_refl _)
               end (eq_refl _)
           end.
   End TABLE_PARSE.
+  End ABS_DERIVS_AND_SPLIT.
+
+  Definition coerce_rng (B B':type) (H:B=B') (A:Type) (f:A->interp B) : A->interp B'.
+    intros B B' H. rewrite H. apply (fun A (f:A->interp B') => f).
+  Defined.
 
   (** At the top-level, we take in a [grammar t], split it into an [astgram] [ag], and 
       fix-up function [f] that maps ASTs from [ag] into [t] values.  Then we build the
@@ -2159,21 +2276,70 @@ Section DFA.
   Definition table_parse n t (g:grammar t) (ts:list token_id) : 
     option ((list token_id) * list (interp t)) := 
     let (ag, f) := split_astgram g in 
-    match build_dfa n ag as d return (build_dfa n ag = d) -> _ with 
+    match build_dfa derivs_and_split n ag as d 
+      return (build_dfa derivs_and_split n ag = d) -> _ with 
       | None => fun _ => None
       | Some d => 
         fun H => 
-          match table_parse' d 0 ts (Xid _) with
+          match table_parse' d _ 0 ts (fun x => x) with
             | None => None
             | Some (existT a' (xf, ts')) => 
               let vs := astgram_extract_nil a' in
-                let xf' := xcoerce xf (eq_refl _) (dfa_zero_coerce _ _ H) in 
-                Some (ts', List.map (fun z => f (xinterp xf' z)) vs)
+                let xf' := coerce_rng (dfa_zero_coerce _ _ _ H) xf in 
+                Some (ts', List.map (fun z => f (xf' z)) vs)
           end
     end (eq_refl _).
 
-End DFA.
+  Record instParserState (t:type) := mkPS { 
+    dfa_ps : DFA ; 
+    row_ps : nat ; 
+    fixup_ps : fixfn ((dfa_states dfa_ps).[row_ps]) t
+  }.
 
+  Definition opt_initial_parser_state (n:nat) t (g:grammar t) : option (instParserState t) := 
+    let (ag, f) := split_astgram g in 
+      match build_dfa derivs_and_split n ag as x 
+        return build_dfa derivs_and_split n ag = x -> option (instParserState t) 
+        with 
+        | None => fun H => None
+        | Some d => fun H => 
+          Some (mkPS d 0 (coerce_dom (eq_sym (dfa_zero_coerce derivs_and_split n ag H)) f))
+      end (eq_refl _).  
+
+  Definition parse_token t (ps:instParserState t) (tk:token_id) : 
+    option (instParserState t * list (interp t)).
+  refine (fun t ps tk => 
+    let d := dfa_ps ps in 
+      match nth_error (dfa_transition d) (row_ps ps) as p return
+        (nth_error (dfa_transition d) (row_ps ps) = p) -> _ 
+        with 
+        | None => fun _ => None
+        | Some row => fun H => 
+          match nth_error (row_entries row) tk as q return
+            (nth_error (row_entries row) tk = q) -> _
+            with 
+            | None => fun _ => None
+            | Some e => fun H' => 
+              let f := next_xform e in 
+              let next_i := next_state e in 
+                if nth next_i (dfa_accepts d) false then
+                  let ag' := nth next_i (dfa_states d) aZero in 
+                    let vs := astgram_extract_nil ag' in 
+                      Some (ps, List.map (fun z => (fixup_ps ps) _) vs)
+                else 
+                  Some (mkPS d next_i (fun z => (fixup_ps ps) _), nil)
+          end (eq_refl _)
+      end (eq_refl _)
+  ) ; generalize (dfa_transition_r d (row_ps ps)) ; rewrite H ; intro g ; rewrite <- g ;
+  apply (f z).
+  Defined.
+
+End DFA.
+Extraction Implicit table_parse [t].
+Extraction Implicit opt_initial_parser_state [t].
+Extraction Implicit parse_token [t].
+
+(*
 (** Alas, the overhead of manipulating the types with the [xform]'s 
     makes the approach developed above unworkable.  In particular,
     the time it takes to construct the DFA table is just too long
@@ -2738,27 +2904,10 @@ Definition thunk {A B} (f:A -> B) (x:A) : memo B := Thunk (fun _ => f x).
 
 (** Now build optimizations for [astgram]s paired with [uform]s as done
     above with [xform]s and prove they are equivalent. *)
-(*
-Definition uassoc_left_sum t1 t2 t3 := 
-  Umatch (Uinl t3 (Uinl t2 Uid))
-         (Umatch (Uinl t3 (Uinr t1 Uid)) 
-                 (Uinr (Thunk (fun _ => Sum_t (force t1) (force t2))) Uid)).
-*)
 
 Fixpoint uappend_alt (ag1 ag2:astgram) : astgram * uform := 
   match ag1 with 
     | aZero => (ag2, Uinr (Val Void_t))
-(*
-   Too expensive to do all the time, so omit.  The longer proof of 
-   equivalence is also commented out below. 
-    | aAlt aga agb => 
-      let (agd, xd) := uappend_alt agb ag2 in 
-        let (agc, xc) := uappend_alt aga agd in 
-          (agc, Ucomp xc (Ucomp (Umatch (Uinl (thunk astgram_type (aAlt agb ag2)) Uid)
-                                        (Uinr (thunk astgram_type aga) xd))
-                                (uassoc_left_sum (thunk astgram_type aga)
-                                  (thunk astgram_type agb) (thunk astgram_type ag2))))
-*)
     | ag1' => 
       match ag2 with 
         | aZero => (ag1', Uinl (Val Void_t))
@@ -2777,44 +2926,11 @@ Proof.
   destruct ag1 ; try (simpl ; auto ; fail) ; 
     try (simpl ; destruct ag2 ; simpl ; auto ; fail).
 Qed.
-(*
-  induction ag1 ; try (simpl ; auto ; fail) ; 
-    try (simpl ; destruct ag2 ; simpl ; auto ; fail).
-  intros. simpl. fold astgram_type. specialize (IHag1_2 ag2).
-  remember (append_alt ag1_2 ag2) as e1 ; destruct e1. destruct IHag1_2 ; subst.
-  specialize (IHag1_1 (fst (uappend_alt ag1_2 ag2))). 
-  remember (append_alt ag1_1 (fst (uappend_alt ag1_2 ag2))) as e2 ; destruct e2. 
-  simpl. destruct IHag1_1. subst. remember (uappend_alt ag1_2 ag2) as e3 ; 
-  destruct e3. simpl in *. remember (uappend_alt ag1_1 a) as e4. destruct e4. 
-  split ; auto. simpl in H1. simpl. rewrite H1. rewrite H0. unfold sumbool_rec, 
-  sumbool_rect. 
-  assert (type_dec (astgram_type ag1_1) (astgram_type ag1_1) = left (eq_refl _)).
-  destruct (type_dec (astgram_type ag1_1) (astgram_type ag1_1)) ; 
-  try congruence. rewrite (proof_irrelevance _ e (eq_refl _)). auto. rewrite H.
-  assert (type_dec (astgram_type ag1_2) (astgram_type ag1_2) = left (eq_refl _)). 
-  destruct (type_dec (astgram_type ag1_2) (astgram_type ag1_2)) ; try congruence.
-  rewrite (proof_irrelevance _ e (eq_refl _)). auto. rewrite H2. simpl.
-  assert (type_dec (astgram_type ag2) (astgram_type ag2) = left (eq_refl _)).
-  destruct (type_dec (astgram_type ag2) (astgram_type ag2)) ; try congruence.
-  rewrite (proof_irrelevance _ e (eq_refl _)). auto. rewrite H3. simpl.
-  rewrite H2. simpl. rewrite H3. simpl. rewrite H. simpl. rewrite H2. simpl.
-  rewrite H3. simpl. uc_simp.
-Qed.
-*)
 
 Fixpoint uappend_cat (ag1 ag2:astgram) : astgram * uform := 
   match ag1 with 
     | aZero => (aZero, Uzero (thunk astgram_type (aCat ag1 ag2)))
     | aEps => (ag2, Upair Uunit Uid)
-(*
-   Too expensive to do all the time, so commented out.  The proof of
-   equivalence for this case is also commented out below. 
-    | aCat aga agb => 
-      let (agd, xd) := uappend_cat agb ag2 in 
-        let (agc, xc) := uappend_cat aga agd in 
-          (agc, Ucomp xc (Ucomp (Upair (Ufst Uid) (Usnd xd)) 
-            (Upair (Upair (Ufst Uid) (Usnd (Ufst Uid))) (Usnd (Usnd Uid)))))
-*)
     | ag1' => 
       match ag2 with 
         | aZero => (aZero, Uzero (thunk astgram_type (aCat ag1' ag2)))
@@ -2834,18 +2950,6 @@ Proof.
   destruct ag1 ; try (simpl ; auto ; fail) ; 
     try (destruct ag2 ; simpl ; auto ; fail).
 Qed.
-(*
-  intros ag1. induction ag1; try (simpl ; auto ; fail) ; 
-  try (destruct ag2 ; simpl ; auto ; fail). intros.
-  simpl. fold astgram_type. specialize (IHag1_2 ag2). remember (append_cat ag1_2 ag2) as e1.
-  destruct e1. destruct IHag1_2 ; subst. specialize (IHag1_1 (fst (uappend_cat ag1_2 ag2))).
-  remember (append_cat ag1_1 (fst (uappend_cat ag1_2 ag2))) as e2. destruct e2.
-  simpl in *. destruct IHag1_1 ; subst. simpl in *.
-  remember (uappend_cat ag1_2 ag2) as e3 ; destruct e3. simpl in *.
-  remember (uappend_cat ag1_1 a) as e4 ; destruct e4. simpl in *. split ; auto. 
-  rewrite H1. rewrite H0. simpl. unfold assoc_left_pair. auto.
-Qed.
-*)
 
 (** Optimize an [astgram], producing a new [astgram] and [uform] *)
 Definition uopt_ag (ag:astgram) : astgram * uform := 
@@ -2853,9 +2957,6 @@ Definition uopt_ag (ag:astgram) : astgram * uform :=
     | aAlt ag1 ag2 => uappend_alt ag1 ag2
     | aCat ag1 ag2 => uappend_cat ag1 ag2
     | aStar aZero => (aEps, Uempty (Val Void_t))
-      (*
-    | aStar (aStar ag') => (aStar ag', Ucons Uid (Uempty (thunk astgram_type (aStar ag'))))
-    *)
     | ag' => (ag', Uid)
   end.
 
@@ -3042,7 +3143,7 @@ Fixpoint uderivs_and_split (ag:astgram) (cs:list char_p) : astgram * uform :=
     | c::cs' => 
       let (ag1, x1) := uderiv_and_split ag c in 
         let (ag2, x2) := uderivs_and_split ag1 cs' in 
-          (ag2, ucomp' x1 x2)
+          (ag2, uopt (ucomp' x1 x2))
   end.
 
 Lemma uderivs_and_split_corr cs ag : 
@@ -3060,9 +3161,176 @@ Proof.
   remember (derivs_and_split (fst (uderiv_and_split ag a)) cs) as e2. destruct e2. 
   destruct IHcs. subst. simpl. remember (uderiv_and_split ag a) as e3. destruct e3.
   simpl in *. remember (uderivs_and_split a0 cs) as e4. destruct e4 ; simpl in *.
-  split ; auto. eapply ucomp'_corr ; auto.
-Qed.
+  split ; auto. generalize (ucomp'_corr _ H0 _ H1). intros.
+
+Check uopt_corr. generalize (uopt_corr (xcomp' x0 x1)). intro. rewrite <- H.
+  assert (H2 : ucomp' u u0 = erase (xcomp' x0 x1)) ; [ idtac | rewrite H2 ; auto ].
   
+Check ucomp'_corr.
+  eapply ucomp'_corr ; auto.
+Qed.
+
+Definition untyped_derivs_and_split (ag:astgram) (cs:list char_p) : 
+  {ag2:astgram & astgram_type ag2 ->> astgram_type ag}.
+  refine (
+    fun ag cs => 
+      match uderivs_and_split ag cs as z return 
+        uderivs_and_split ag cs = z -> {ag2:astgram & astgram_type ag2 ->> astgram_type ag}
+        with 
+          | (ag2,u) => 
+            fun H1 => 
+              match decorate (astgram_type ag2) u as d 
+                return (decorate (astgram_type ag2) u = d) ->   
+                {ag2:astgram & astgram_type ag2 ->> astgram_type ag}
+                with 
+                | None => fun H => _
+                | Some (existT t x) => 
+                  fun H => 
+                    existT (fun ag0 => astgram_type ag0 ->> astgram_type ag) ag2 _
+              end (eq_refl (decorate (astgram_type ag2) u))
+      end (eq_refl (uderivs_and_split ag cs))
+      ). 
+  assert (t = astgram_type ag).
+  generalize (uderivs_and_split_corr cs ag). rewrite H1. simpl.
+  destruct (derivs_and_split ag cs). intros. destruct H0.
+  subst. rewrite H in H2. uc_simp. rewrite <- H0. apply x.
+  assert False.
+  generalize (uderivs_and_split_corr cs ag). rewrite H1. simpl.
+  destruct (derivs_and_split ag cs). intros. destruct H0. subst.
+  congruence. contradiction.
+Defined.
+
+Definition cast_memo (m1 m2:memo type) (H:m1=m2) : interp (force m1) -> interp (force m2).
+  intros m1 m2 H. rewrite H. apply (fun x => x).
+Defined.
+
+Definition uinterp (m1:memo type) (u:uform) :
+  option {m2 : memo type & interp (force m1) -> interp (force m2)}.
+refine (fix uinterp (m1:memo type) (u:uform) {struct u} :
+  option {m2 : memo type & interp (force m1) -> interp (force m2)} := 
+  match u with 
+    | Uid => Some (existT _ m1 (fun x => x))
+    | Uzero m => 
+      match (force m1) as t1 return option {m2:memo type & interp t1 -> interp (force m2)}
+        with 
+        | Void_t => Some (existT _ m (fun (x:interp Void_t) => match x with end))
+        | _ => None
+      end
+    | Ucomp u1 u2 => 
+      match uinterp m1 u1 with 
+        | None => None
+        | Some (existT m2 f1) => 
+          match uinterp m2 u2 with 
+            | None => None
+            | Some (existT m3 f2) => 
+              Some
+                (existT
+                   (fun m4 => interp (force m1) -> interp (force m4)) m3
+                   (fun x : interp (force m1) => f2 (f1 x)))
+          end
+      end
+    | Uchar c => 
+      Some (existT (fun m4 => interp (force m1) -> interp (force m4)) 
+        (Val Char_t) (fun x : interp (force m1) => c))
+    | Uunit => 
+      Some (existT (fun m4 => interp (force m1) -> interp (force m4)) 
+        (Val Unit_t) (fun x : interp (force m1) => tt))
+    | Uempty m => 
+      Some (existT (fun m4 => interp (force m1) -> interp (force m4)) 
+        (Thunk (fun _ => List_t (force m))) (fun x : interp (force m1) => nil))
+    | Upair u1 u2 => 
+      match uinterp m1 u1 with 
+        | None => None
+        | Some (existT ma fa) => 
+          match uinterp m1 u2 with 
+            | None => None
+            | Some (existT mb fb) => 
+              Some (existT (fun m4 => interp (force m1) -> interp (force m4))
+                (Thunk (fun _ => Pair_t (force ma) (force mb)))
+                (fun x : interp (force m1) => (fa x, fb x)))
+          end
+      end
+    | Ufst => 
+      match force m1 as t1 return option {m2:memo type & interp t1 -> interp (force m2)}
+        with 
+        | Pair_t ta tb => 
+          Some (existT (fun m4 => interp (Pair_t ta tb) -> interp (force m4))
+            (Val ta) (fun x => fst x))
+        | _ => None
+      end
+    | Usnd => 
+      match force m1 as t1 return option {m2:memo type & interp t1 -> interp (force m2)}
+        with 
+        | Pair_t ta tb => 
+          Some (existT (fun m4 => interp (Pair_t ta tb) -> interp (force m4))
+            (Val tb) (fun x => snd x))
+        | _ => None
+      end
+    | Uinl m => 
+      Some (existT (fun m4 => interp (force m1) -> interp (force m4)) 
+        (Thunk (fun _ => Sum_t (force m1) (force m))) (fun x : interp (force m1) => inl x))
+    | Uinr m => 
+      Some (existT (fun m4 => interp (force m1) -> interp (force m4)) 
+        (Thunk (fun _ => Sum_t (force m) (force m1))) (fun x : interp (force m1) => inr x))
+    | Umatch u1 u2 => 
+      match force m1 as t1 return option {m2:memo type & interp t1 -> interp (force m2)}
+        with 
+        | Sum_t ta tb => 
+          match uinterp (Val ta) u1 with 
+            | None => None
+            | Some (existT t1 f1) => 
+              match uinterp (Val tb) u2 with 
+                | None => None
+                | Some (existT t2 f2) => 
+                  match type_dec (force t1) (force t2) with 
+                    | left H => 
+                      Some (existT (fun m4 => interp (Sum_t ta tb) -> interp (force m4)) 
+                        t1 (fun x : interp (Sum_t ta tb) => 
+                             match x with 
+                               | inl a => f1 a
+                               | inr b => _
+                             end))
+                    | right H => None
+                  end
+              end
+          end
+        | _ => None
+      end
+    | Ucons u1 u2 => 
+      match uinterp m1 u1 with 
+        | None => None
+        | Some (existT t1 f1) => 
+          match uinterp m1 u2 with 
+            | None => None
+            | Some (existT t2 f2) => 
+              match type_dec (List_t (force t1)) (force t2) with 
+                | left H => 
+                  Some (existT (fun m4 => interp (force m1) -> interp (force m4)) 
+                    (Thunk (fun _ => (List_t (force t1))))
+                    (fun x : interp (force m1) => (f1 x) :: _))
+                | right H => None
+              end
+          end
+      end
+    | Umap u' => 
+      match force m1 as t1 return option {m2:memo type & interp t1 -> interp (force m2)}
+        with 
+        | List_t t => 
+          match uinterp (Val t) u' with 
+            | None => None
+            | Some (existT t2 f) => 
+              Some (existT (fun m4 => interp (List_t t) -> interp (force m4)) 
+                (Thunk (fun _ => List_t (force t2)))
+                (fun x : interp (List_t t) => List.map f x))
+          end
+        | _ => None
+      end
+  end
+). rewrite H. apply (f2 b).
+assert (interp (List_t (force t1)) = interp (force t2)).
+rewrite H. auto. simpl in H0. rewrite H0. apply (f2 x).
+Defined.
+
 (** Construction of "untyped" DFA. *)
 Section UDFA.
   Notation "s .[ i ] " := (nth i s aZero) (at level 40).
@@ -3092,9 +3360,10 @@ Section UDFA.
         | 0 => (nil, nil)
         | S n' => 
           let (g', u) := uderivs_and_split g (token_id_to_chars tid) in 
+            let uo := uopt u in 
             let p := find_or_add g' s in 
               let (s2, row) := ugen_row' n' (1 + tid) (s ++ (fst p))  in
-              let e : uentry_t := {| unext_state := (snd p) ; unext_uform := uopt u |} in
+              let e : uentry_t := {| unext_state := (snd p) ; unext_uform := uo |} in
                 ((fst p) ++ s2, e::row)
       end.
     Definition ugen_row (s:states_t) : states_t * urow_t := 
@@ -3178,18 +3447,21 @@ Section UDFA.
         | None => None
         | Some (ag', u, ts') => 
           let vs := astgram_extract_nil ag' in 
-            match decorate (astgram_type ag') u with
+            match uinterp (Thunk (fun _ => astgram_type ag')) u with 
               | None => None
-              | Some (existT t' x) => 
-                match type_dec t' (astgram_type ag) with
+              | Some (existT m' f) => 
+                match type_dec (force m') (astgram_type ag) with 
                   | right _ => None
                   | left H => 
-                    let xf' : xform (astgram_type ag') (astgram_type ag) := 
-                      xcoerce x (eq_refl _) H in
-                      Some (ts', List.map (fun z => xinterp xf' z) vs)
+                    let xf' : interp (astgram_type ag') -> interp (astgram_type ag) := 
+                      (eq_rect (force m')
+                        (fun t : type => interp (astgram_type ag') -> interp t) f 
+                        (astgram_type ag) H)
+                      in 
+                      Some (ts', List.map xf' vs)
                 end
             end
-      end.
+      end. 
   End UTABLE_PARSE. 
 
   (** Given some fuel [n] and a grammar [g] of type [t], splits [g] into 
@@ -3211,7 +3483,6 @@ Section UDFA.
                     end)
         end.
 
-
   Record instParserState (t:type) := mkPS {
     udfa : UDFA;  (* the untyped parser table *)
     agram: astgram; (* the original astgram after spliting *)
@@ -3219,6 +3490,12 @@ Section UDFA.
 
     row : nat;  (* the current astgram *)
     uf : uform (* the untyped transform *)
+  }.
+
+  Record t_instParserState (t:type) := mkt_PS {
+    t_dfa : DFA;  (* the untyped parser table *)
+    t_row : nat;  (* the current astgram *)
+    t_f : interp (astgram_type (nth t_row (dfa_states t_dfa) aZero)) -> interp t
   }.
 
   Definition opt_initial_parser_state n t (g:grammar t)
@@ -3229,6 +3506,49 @@ Section UDFA.
           | Some d => Some (mkPS d f 0 Uid)
         end.
 
+  Definition t_opt_initial_parser_state n t (g:grammar t) : option (t_instParserState t) :=
+    let (ag, f) := split_astgram g in 
+      match build_dfa untyped_derivs_and_split n ag as z 
+        return (build_dfa untyped_derivs_and_split n ag = z) -> _ with 
+        | None => fun H => None
+        | Some d => fun H => 
+          Some (mkt_PS t d 0 
+            (eq_rect_r
+              (fun a => interp (astgram_type a) -> interp t) f
+               (build_dfa_zero untyped_derivs_and_split n ag H)))
+      end (eq_refl _).
+
+  Definition t_parse_token t (ps:t_instParserState t) (tk:token_id) :
+    option (t_instParserState t * list (interp t)).
+  refine (fun t ps tk => 
+    let d := t_dfa ps in 
+      match nth_error (dfa_transition d) (t_row ps) as p return 
+        (nth_error (dfa_transition d) (t_row ps) = p) -> _
+        with
+        | None => fun _ => None
+        | Some row => 
+          fun H => 
+          match nth_error (row_entries row) tk as q return 
+            (nth_error (row_entries row) tk = q) -> _
+            with 
+            | None => fun _ => None
+            | Some e => 
+              fun H' => 
+              let f := next_xform e in
+              let next_i := next_state e in
+                if nth next_i (dfa_accepts d) false then
+                  (* get to an acceptance state *)
+                  let ag' := nth next_i (dfa_states d) aZero in
+                    let vs := astgram_extract_nil ag' in 
+                      Some (ps, List.map (fun z => (t_f ps) _) vs)
+                else
+                  Some (mkt_PS t d next_i (fun z => (t_f ps) _),nil)
+          end (eq_refl _)
+      end (eq_refl _)) ; 
+    generalize (dfa_transition_r d) ; intro g ; specialize (g (t_row ps)) ;
+    rewrite H in g ; rewrite <- g ; apply (f z).
+  Defined.
+  
   Definition parse_token t (ps:instParserState t) (tk:token_id) : 
     option (instParserState t * list (interp t)) := 
     let d := udfa ps in
@@ -3265,5 +3585,6 @@ Section UDFA.
       end.
 
   End UDFA.
-
-End NewParser.
+*)
+(*End NewParser.*)
+(*End X86_BASE_PARSER.*)
